\subsection{Lecture 12}

\begin{lemma}[lemma 3]\label{lemma 3}
   Let \( A  \) be a subset of \( \R  \) and \( f,g : A \in \R  \) be two bounded functions. Then 
   \begin{enumerate}
       \item[(i)] \( \sup_{A} (f+g) \leq \sup_{A} f + \sup_{A} g \);
       \item[(ii)] \( \inf_{A} (f+g) \geq \inf_{A} f + \inf_{A} g  \);
       \item[(iii-1)] \( \forall k \geq 0  \), \( \sup_{A} (kf) = k \sup_{A} f \);
       \item[(iii-2)] \(  \forall k \geq 0  \) \( \inf_{A} kf = k \inf_{A} f \);
       \item[(iv-1)] \( \forall k < 0  \) \( \sup_{A} kf = k \inf_{A} f \); 
       \item[(iv-2)] \( \forall k < 0  \) \( \inf_{A} kf = k \sup_{A} f \);
       \item[(v)] \( \sup_{x,y \in A}| f(x) - f(y) | = \sup_{A} f - \inf_{A} f \);
        \item[(vi)] If there exists a constant \( k > 0  \) such that 
            \[  \forall z,w \in A \ \ | f(z) - f(w)  | \leq k | g(z) - g(w) |,  \]
            then
            \[  \sup_{A} f - \inf_{A} f \leq k [\sup_{A} g - \inf_{A}  g].  \]
   \end{enumerate}  
\end{lemma}

\begin{lemma}[lemma 4]\label{lemma 4}
    Let \( f,g: [a,b] \to \R  \) be two bounded functions, \( \alpha: [a,b] \to \R  \) is an increasing function, and \( P \in \Pi[a,b] \). Then
    \begin{enumerate}
        \item[(i)] \( U(f + g,\alpha, P) \leq U(f,\alpha,P) + U(g,\alpha,P) \);
        \item[(ii)] \( L(f+g, \alpha, P) \geq L(f,\alpha,P) + U(g,\alpha, P) \);
        \item[(iii-1)] \( \forall k \geq 0  \) \( U(kf, \alpha, P) = k U(f,\alpha,P) \)
        \item[(iii-2)] \( \forall k \geq 0  \), \( L(kf,\alpha,P) = k L(f,\alpha,P) \);
        \item[(iv-1)] \( \forall k < 0  \) \( U(f,\alpha,P) = k L(f,\alpha,P) \)
        \item[(iv-2)] \( \forall k < 0  \) \( L(kf,\alpha, P) = k U(f,\alpha,P) \).
    \end{enumerate}
\end{lemma}

\begin{theorem}[Order Properties of R.S Integral]\label{Order properties of R.S integrals} 
    Assume \( f,g \in {R}_{\alpha}[a,b] \). Then
    \begin{enumerate}
        \item[(i)] If \( m \leq f(x) \leq M  \) for all \( x\in [a,b] \), then 
            \[  m (\alpha(b) - \alpha(a)) \leq \int_{ a }^{ b }  f  \ d \alpha \leq M(\alpha(b) - \alpha(a)). \]
        \item[(ii)] If \( f \leq g  \) on \( [a,b] \), then
            \[  \int_{ a }^{ b }  f  \ d \alpha \leq \int_{ a }^{ b } g   \ d \alpha. \]
    \end{enumerate}
\end{theorem}
\begin{proof}
\begin{enumerate}
    \item[(i)] Note that for any \( P \in \Pi[a,b] \), we have 
        \begin{align*}
            \int_{ a }^{ b }  f  \ d \alpha &= L(f,\alpha) \geq L(f,\alpha,P) \\
            \int_{ a }^{ b }  f \ d \alpha &= U(f,\alpha) \leq U(f,\alpha,P).
        \end{align*}
        In particular, for the partition \( P = \{ a,b \}  \), we have 
        \begin{align*}
            \int_{ a }^{ b }  f  \ d \alpha &\geq L(f,\alpha, P) = \Big(  \inf_{x \in [a,b]} f(x) \Big) (\alpha(b) - \alpha(a)) \geq m (\alpha(b) - \alpha(a)) \tag{1} \\
            \int_{ a }^{ b }  f  \ d \alpha &\leq U(f,\alpha,P) = \Big(  \sup_{x \in [a,b]} f(x) \Big) (\alpha(b) - \alpha(a)) \leq M (\alpha(b) - \alpha(a)). \tag{2}
        \end{align*}
        Using (1) and (2), we obtain our desired result.
    \item[(ii)] Let \( h = g - f  \). We have \( h \geq 0  \), so, by part (i), we have
        \[  0 (\alpha(b) - \alpha(a)) \leq \int_{ a }^{ b }  h  \ d \alpha. \]
        Therefore, 
        \begin{align*}
            0 \leq \int_{ a }^{ b } h \ d \alpha &= \int_{ a }^{ b } g - f  \ d \alpha = \int_{ a }^{ b }  g  \ d \alpha - \int_{ a }^{ b }  f  \ d \alpha \\
                                                 &\implies \int_{ a }^{ b } f  \ d \alpha \leq \int_{ a }^{ b }  g  \ d \alpha.
        \end{align*}
\end{enumerate}
\end{proof}

\begin{theorem}[Triangle Inequality of Integrals]
    Assume \( f \in {R}_{\alpha}[a,b] \). Then
    \begin{enumerate}
        \item[(i)] \( | f |  \in {R}_{\alpha}[a,b] \);
        \item[(ii)] \( \displaystyle \Big| \int_{ a }^{ b }  f  \ d \alpha \Big|  \leq \int_{ a }^{ b }  | f |  \ d \alpha \).
    \end{enumerate}
\end{theorem}
\begin{proof}
\begin{enumerate}
    \item[(i)] Define \( \varphi: \R \to \R  \) by \( \varphi(x) = | x  |  \) which is clearly continuous on \( \R  \). Since \( f \in {R}_{\alpha}[a,b] \), it follows from {\hyperref[Rudin 6.11]{Rudin 6.11}} that \( \varphi \circ f \in {R}_{\alpha}[a,b] \). Hence, we have \( | f |  \in {R}_{\alpha}[a,b]  \).  
    \item[(ii)] Recall that 
        \[  | t  |  \leq s \iff - s \leq t \leq s.  \]
        So, our goal is to show that 
        \[ - \int_{ a }^{ b }  | f  |  \ d \alpha \leq \int_{ a }^{ b }  f  \ d \alpha \leq \int_{ a }^{ b }  | f  |  \ d \alpha. \]
        Also, we have 
        \[ - | f(x) |  \leq f(x) \leq | f(x) |  \ \ \forall x \in [a,b].  \]
        So, 
        \[  -\int_{ a }^{ b }  | f(x) |  \ d \alpha \leq \int_{ a }^{ b }  f(x) \ d \alpha \leq \int_{ a }^{ b }  | f(x) |  \ d \alpha \]
        as desired.
\end{enumerate}
\end{proof}



